more transpose, some stuff about dfs ordering, figuring out graph ordering

SCCAlg.v
@@ -11,7 +11,114 @@ Require Import Omega.
 Require Import Coq.FSets.FSetProperties.
 Require Import DerivedProofs.
 Require Import SCCDef.
+Require Import Coq.Classes.RelationClasses.
 
+(*In reality, our graoh is fixed, but Coq's modules do not seem to support a value parameter*)
+Module ReverseFTime (O: UsualOrderedType)(S: FSetInterface.Sfun O)(G: Graph O S)(F: Forest O S G)
+  (D: DFSBase O S G F) <: OrderedType.
+
+  Definition t : Type := {x : G.graph * G.vertex | G.contains_vertex (fst x) (snd x) = true}.
+
+  Definition eq (t1 t2 : t) := if G.Equal_dec (fst (proj1_sig t1)) (fst (proj1_sig t2)) then
+    D.f_time None (fst (proj1_sig t1)) (snd (proj1_sig t1)) = 
+         D.f_time None (fst (proj1_sig t2)) (snd (proj1_sig t2)) 
+    else False.
+
+  Definition lt (t1 t2 : t) :=
+    if G.Equal_dec (fst (proj1_sig t1)) (fst (proj1_sig t2)) 
+    then D.f_time None (fst (proj1_sig t1)) (snd (proj1_sig t1)) > 
+         D.f_time None (fst (proj1_sig t2)) (snd (proj1_sig t2)) 
+    else G.lt (fst (proj1_sig t1)) (fst (proj1_sig t2)).
+
+  Lemma eq_refl : forall x : t, eq x x.
+  Proof.
+    intros. unfold eq. destruct x as [x H]. destruct x as [g v]. simpl in *.
+    destruct (G.Equal_dec g g). omega. apply n. pose proof (G.Equal_equiv).
+    destruct H0 as [refl]. apply refl.
+  Qed.
+  
+  Lemma eq_sym : forall x y : t, eq x y -> eq y x.
+  Proof.
+    intros. unfold eq in *. destruct x as [x1 H1]. destruct y as [y1 H2]. destruct x1 as [g1 v1].
+    destruct y1 as [g2 v2]. simpl in *. pose proof (G.Equal_equiv). destruct H0 as [refl sym trans].
+    destruct (G.Equal_dec g2 g1). destruct (G.Equal_dec g1 g2). omega. 
+    apply sym in e. contradiction. destruct (G.Equal_dec g1 g2). apply sym in e. contradiction. apply H.
+  Qed.
+
+  Lemma eq_trans : forall x y z : t, eq x y -> eq y z -> eq x z.
+  Proof.
+    intros. unfold eq in *. destruct x as [x1 H1]. destruct y as [y1 H2]. destruct z as [z1 H3].
+    destruct x1 as [g1 v1]. destruct y1 as [g2 v2]. destruct z1 as [g3 v3]. simpl in *.
+    pose proof (G.Equal_equiv). destruct H4 as [refl sym trans].
+    destruct (G.Equal_dec g1 g3). destruct (G.Equal_dec g1 g2). destruct (G.Equal_dec g2 g3). omega.
+    assert (G.Equal g2 g3). eapply trans. apply sym. apply e0. apply e. contradiction.
+    destruct H. destruct (G.Equal_dec g1 g2). destruct (G.Equal_dec g2 g3).
+    assert (G.Equal g1 g3). eapply trans. apply e. apply e0. contradiction. destruct H0. destruct H.
+  Qed. 
+
+  Lemma lt_trans : forall x y z : t, lt x y -> lt y z -> lt x z.
+  Proof.
+    intros. destruct x. destruct y. destruct z. unfold lt in *. simpl in *.
+    destruct x as [g1 v1]. destruct x0 as [g2 v2]. destruct x1 as [g3 v3]. simpl in *.
+     pose proof G.Equal_equiv. destruct H1 as [refl sym trans].
+    destruct (G.Equal_dec g1 g2). destruct (G.Equal_dec g2 g3). 
+    destruct (G.Equal_dec g1 g3). omega.
+    assert (G.Equal g1 g3). eapply trans. apply e2. apply e3. contradiction.
+    destruct (G.Equal_dec g1 g3). assert (G.Equal g2 g3). eapply trans. eapply sym. apply e2.
+    apply e3. contradiction. eapply G.Equal_lt_l. apply e2. apply H0.
+    destruct (G.Equal_dec g1 g3). destruct (G.Equal_dec g2 g3). 
+    assert (G.Equal g1 g2). eapply trans. apply e2. apply sym. apply e3. contradiction.
+    assert (G.lt g2 g1). eapply G.Equal_lt_r. apply e2. apply H0.
+    assert (G.lt g1 g1). eapply G.lt_trans. apply H. apply H1. eapply G.lt_not_eq in H2.
+    exfalso. apply H2. apply refl. destruct (G.Equal_dec g2 g3). eapply G.Equal_lt_r. apply sym.
+    apply e2. apply H. eapply G.lt_trans. apply H. apply H0.
+  Qed.
+
+ Lemma lt_not_eq : forall x y : t, lt x y -> ~ eq x y.
+  Proof.
+    intros. intro. unfold lt in *. unfold eq in *. destruct x as [x A]. simpl in *.
+    destruct y as [y B]. destruct x as [g v]. destruct y as [g' v']. simpl in *.
+    destruct (G.Equal_dec g g'). omega. apply H0.
+  Qed.
+
+ Definition compare : forall x y : t, Compare lt eq x y.
+  Proof.
+    intros. destruct x as [x1 H1]. destruct y as [y1 H2]. destruct x1 as [g1 v1]. destruct y1 as [g2 v2].
+    simpl in *. pose proof (G.Equal_equiv). destruct H as [r s t]. 
+    pose proof (G.compare g1 g2). destruct H.
+    - apply LT. unfold lt. simpl in *. destruct (G.Equal_dec g1 g2). apply G.lt_not_eq in l. 
+      contradiction. apply l.
+    - case_eq (Nat.compare (D.f_time None g1 v1) (D.f_time None g2 v2)); intro; simpl in *.
+      + apply EQ. unfold eq. simpl in *. destruct (G.Equal_dec g1 g2). apply nat_compare_eq in H. omega.
+        contradiction.
+      + apply GT. unfold lt. simpl in *. destruct (G.Equal_dec g2 g1). apply nat_compare_lt in H. omega.
+        apply s in e. contradiction.
+      + apply LT. unfold lt. simpl in *. destruct (G.Equal_dec g1 g2). apply nat_compare_gt in H. omega.
+        contradiction.
+    - apply GT. unfold lt. simpl in *. destruct (G.Equal_dec g2 g1). apply G.lt_not_eq in l. contradiction.
+      apply l.
+  Qed.
+
+ Lemma eq_dec : forall x y : t, { eq x y } + { ~ eq x y }.
+  Proof.
+    intros. pose proof (compare x y). destruct H. right. intro. apply lt_not_eq in l. contradiction.
+    left. apply e. right. intro. apply lt_not_eq in l. apply eq_sym in H. contradiction.
+  Qed.
+
+End ReverseFTime.
+
+ Parameter Inline t : Type.
+ Definition eq := @eq t.
+ Parameter Inline lt : t -> t -> Prop.
+ Definition eq_refl := @eq_refl t.
+ Definition eq_sym := @eq_sym t.
+ Definition eq_trans := @eq_trans t.
+ Axiom lt_trans : forall x y z : t, lt x y -> lt y z -> lt x z.
+ Axiom lt_not_eq : forall x y : t, lt x y -> ~ eq x y.
+ Parameter compare : forall x y : t, Compare lt eq x y.
+ Parameter eq_dec : forall x y : t, { eq x y } + { ~ eq x y }.
+
+*)
 Module SCCAlg(O: UsualOrderedType)(S: FSetInterface.Sfun O)(G: Graph O S)(F: Forest O S G)(D: DFSBase).
 
   Module Pa := (Path.PathTheories O S G).
@@ -20,6 +127,8 @@ Module SCCAlg(O: UsualOrderedType)(S: FSetInterface.Sfun O)(G: Graph O S)(F: For
   Module SN := Helper.SetNeq O S.
   Module SC := SCCDef.SCCDef O S G.
   Import SC.
+
+Search S.Equal.
 
 (** Correctness of SCC algorithm **)
 
@@ -420,6 +529,29 @@ Proof.
     split. eapply min_elt_set_in_set. apply H5. eapply min_elt_set_in_set. apply H6.
     apply A. apply B.
 Qed.
+
+(*Corollary 22.15 in CLRS*)
+Lemma scc_finish_time_transpose: forall g c c' u v (Hc: scc c g) (Hc': scc c' g) x y,
+  S.equal c c' = false ->
+  G.contains_edge (G.get_transpose g) u v = true ->
+  S.In u c ->
+  S.In v c' ->
+  f_time_scc g c Hc = Some x ->
+  f_time_scc g c' Hc' = Some y ->
+  D1.f_time None g x < D1.f_time None g y.
+Proof.
+  intros. assert (D1.f_time None g x < D1.f_time None g y <-> D1.f_time None g y > D1.f_time None g x) by omega.
+  rewrite H5. clear H5. eapply scc_finish_time. assert (S.equal c' c = false). destruct (S.equal c' c) eqn : ?.
+  apply S.equal_2 in Heqb. rewrite Heqb in H. assert (~S.Equal c c). intro. 
+  apply SCCAlg.P2.FM.equal_iff in H5. rewrite H5 in H. inversion H.
+  pose proof (P2.equal_refl c). contradiction. reflexivity. apply H5.
+  rewrite G.transpose_edges. apply H0. apply H2. apply H1. apply H4. apply H3.
+Qed.
+
+(** Defining the second DFS pass **)
+
+
+
 
 End SCCAlg.
 
